oh my. there was an admit there, now using the possible types technique. we prolly do not need layered trans here, but it was hard to keep the proof flavor without value inversion

stable/FsubL_alt.v
@@ -1327,6 +1327,19 @@ Proof.
   apply* sub_transitivity.
 Qed.
 
+Lemma sub_narrowing_empty : forall Q0 Q1 m Z P0 P1 S T,
+  sub oktrans empty Q0 P0 ->
+  sub oktrans empty P1 Q1 ->
+  sub m (Z ~ bind_sub Q0 Q1) S T ->
+  sub m (Z ~ bind_sub P0 P1) S T.
+Proof.
+  intros.
+  rewrite <- (concat_empty_r (Z ~ bind_sub P0 P1)).
+  rewrite <- (concat_empty_l (Z ~ bind_sub P0 P1)).
+  apply* sub_narrowing.
+  rewrite concat_empty_r. rewrite concat_empty_l. auto.
+Qed.
+
 Inductive notvar : typ -> Prop :=
   | notvar_top   : notvar typ_top
   | notvar_bot   : notvar typ_bot
@@ -1371,11 +1384,23 @@ Proof.
       eauto.
 Qed.
 
-Lemma sub_trans_pushback : forall E T1 T3,
-  sub oktrans E T1 T3 ->
-  sub notrans E T1 T3.
+Lemma sub_trans_pushback_empty : forall T1 T3,
+  sub oktrans empty T1 T3 ->
+  sub notrans empty T1 T3.
 Proof.
-Admitted.
+  introv Hst. remember empty as E. generalize dependent HeqE.
+  induction Hst; intros; subst; eauto.
+  false. apply* binds_empty_inv.
+  false. apply* binds_empty_inv.
+  apply_fresh* sub_all as Y.
+  assert (wft empty T2) as HwfT2 by auto.
+  assert (notvar T2) as N. {
+    inversion HwfT2; subst; auto.
+    inversion HwfT2; subst.
+    false. apply* binds_empty_inv.
+  }
+  eapply sub_trans_notvar. apply N. eapply IHHst1; eauto. eapply IHHst2; eauto.
+Qed.
 
 End NarrowTrans.
 
@@ -1386,20 +1411,20 @@ Lemma sub_through_subst_tt : forall Q0 Q1 m F Z S T P,
   sub m (Z ~ bind_sub Q0 Q1 & F) S T ->
   sub oktrans empty Q0 P ->
   sub oktrans empty P Q1 ->
-  sub m (map (subst_tb Z P) F) (subst_tt Z P S) (subst_tt Z P T).
+  sub oktrans (map (subst_tb Z P) F) (subst_tt Z P S) (subst_tt Z P T).
 Proof.
   introv SsubT Q0subP PsubQ1. lets R: (sub_regular Q0subP).
   destruct R as [_ [_ Pwf]].
   inductions SsubT; introv; simpl subst_tt.
-  apply* sub_top.
-  apply* sub_bot.
+  apply sub_trans_ok. apply* sub_top.
+  apply sub_trans_ok. apply* sub_bot.
   case_var.
     apply* sub_reflexivity. apply* wft_weaken_empty.
     apply* sub_reflexivity.
     inversions H0. binds_cases H3.
       apply* (@wft_var (subst_tt Z P T0) (subst_tt Z P T1)). unsimpl_map_bind_sub*.
   case_var.
-    apply sub_trans_pushback. apply (@sub_transitivity Q1).
+    apply (@sub_transitivity Q1).
       apply_empty* sub_weakening_empty.
       rewrite* <- (@subst_tt_fresh Z P Q1).
         rewrite <- concat_empty_l in H. rewrite concat_assoc in H. binds_get H.
@@ -1407,10 +1432,10 @@ Proof.
         eapply sub_regular. eauto.
         inversion H0. subst. auto*.
         apply* (@notin_fv_wf empty).
-    apply* (@sub_trans_tvar (subst_tt Z P T0) (subst_tt Z P T1)).
+    apply sub_trans_ok. apply* (@sub_trans_tvar (subst_tt Z P T0) (subst_tt Z P T1)).
         binds_cases H; unsimpl_map_bind_sub*.
   case_var.
-    apply sub_trans_pushback. apply (@sub_transitivity Q0).
+    apply (@sub_transitivity Q0).
     rewrite* <- (@subst_tt_fresh Z P Q0).
     rewrite <- concat_empty_l in H. rewrite concat_assoc in H. binds_get H.
     rewrite concat_empty_l. apply ok_from_okt. eapply proj1.
@@ -1418,15 +1443,15 @@ Proof.
     inversion H0. subst. auto*.
     apply* (@notin_fv_wf empty).
     apply_empty* sub_weakening_empty.
-    apply* (@sub_trans_tvar_lower (subst_tt Z P T0) (subst_tt Z P T1)).
+    apply sub_trans_ok. apply* (@sub_trans_tvar_lower (subst_tt Z P T0) (subst_tt Z P T1)).
     binds_cases H; unsimpl_map_bind_sub*.
-  apply* sub_arrow.
-  apply* sub_refl_all.
+  apply sub_trans_ok. apply* sub_arrow.
+  apply sub_trans_ok. apply* sub_refl_all.
    change (typ_all (subst_tt Z P T0) (subst_tt Z P T1) (subst_tt Z P T2))
           with
           (subst_tt Z P (typ_all T0 T1 T2)).
    auto*.
-  apply_fresh* sub_all as X.
+  apply sub_trans_ok. apply_fresh* sub_all as X.
    unsimpl (subst_tb Z P (bind_sub T0 T1)).
    repeat rewrite* subst_tt_open_tt_var.
    assert (map (subst_tb Z P) F & X ~ subst_tb Z P (bind_sub T0 T1) =
@@ -1434,9 +1459,10 @@ Proof.
      rewrite map_concat. rewrite map_single. reflexivity.
    }
    rewrite A. apply* H0. rewrite concat_assoc. reflexivity.
-  apply* sub_trans_ok.
+  apply* IHSsubT.
   apply* sub_trans.
 Qed.
+
 
 (* ********************************************************************** *)
 (** * Properties of Typing *)
@@ -1506,6 +1532,20 @@ Proof.
   apply* typing_sub. apply* (@sub_narrowing Q0 Q1).
 Qed.
 
+Lemma typing_narrowing_empty : forall Q0 Q1 X P0 P1 e T,
+  sub oktrans empty Q0 P0 ->
+  sub oktrans empty P1 Q1 ->
+  sub oktrans empty P0 P1 ->
+  typing (X ~ bind_sub Q0 Q1) e T ->
+  typing (X ~ bind_sub P0 P1) e T.
+Proof.
+  intros.
+  rewrite <- (concat_empty_r (X ~ bind_sub P0 P1)).
+  rewrite <- (concat_empty_l (X ~ bind_sub P0 P1)).
+  apply* typing_narrowing.
+  rewrite concat_empty_r. rewrite concat_empty_l. auto.
+Qed.
+
 (************************************************************************ *)
 (** Preservation by Term Substitution (8) *)
 
@@ -1572,44 +1612,157 @@ Qed.
 (* ********************************************************************** *)
 (** Inversions for Typing (13) *)
 
-Lemma typing_inv_abs : forall E S1 e1 T,
-  typing E (trm_abs S1 e1) T ->
-  forall U1 U2, sub notrans E T (typ_arrow U1 U2) ->
-     sub oktrans E U1 S1
-  /\ exists S2, exists L, forall x, x \notin L ->
-     typing (E & x ~ bind_typ S1) (e1 open_ee_var x) S2 /\ sub oktrans E S2 U2.
+Inductive possible_types : trm -> typ -> Prop :=
+| pt_top : forall v, value v -> possible_types v typ_top
+| pt_arrow : forall L V V' e1 T1 T1',
+  (forall x, x \notin L -> typing (x ~ bind_typ V) (e1 open_ee_var x) T1) ->
+  sub oktrans empty V' V ->
+  sub oktrans empty T1 T1' ->
+  possible_types (trm_abs V e1) (typ_arrow V' T1')
+| pt_all : forall L VS VS' VU VU' e1 T1 T1',
+  (forall X, X \notin L -> typing (X ~ bind_sub VS VU) (e1 open_te_var X) (T1 open_tt_var X)) ->
+  sub oktrans empty VS VS' ->
+  sub oktrans empty VU' VU ->
+  (forall X, X \notin L -> sub oktrans (X ~ bind_sub VS' VU') (T1 open_tt_var X) (T1' open_tt_var X)) ->
+  possible_types (trm_tabs VS VU e1) (typ_all VS' VU' T1')
+.
+
+Lemma possible_types_closure : forall v T U,
+  possible_types v T ->
+  sub notrans empty T U ->
+  possible_types v U.
 Proof.
-  introv Typ. gen_eq e: (trm_abs S1 e1). gen S1 e1.
-  induction Typ; intros S1 b1 EQ U1 U2 Sub; inversions EQ.
-  inversions* Sub. auto* (@sub_transitivity T) sub_trans_ok sub_trans_pushback.
+  introv Hpt Hsub. generalize dependent U. induction Hpt; intros.
+  - inversion Hsub; subst.
+    + eapply pt_top; eauto.
+    + false. eapply binds_empty_inv; eauto.
+  - inversion Hsub; subst.
+    + eapply pt_top; eauto. eapply value_abs; eauto.
+      apply_fresh term_abs as y; eauto.
+      assert (y \notin L) as Fr by eauto.
+      specialize (H y Fr).
+      eapply typing_regular in H. destruct H as [? [A ?]].
+      eapply A.
+    + false. eapply binds_empty_inv; eauto.
+    + eapply pt_arrow; eauto.
+      eapply sub_trans; eauto.
+      eapply sub_trans; eauto.
+  - inversion Hsub; subst.
+    + eapply pt_top; eauto. eapply value_tabs; eauto.
+      apply_fresh term_tabs as Y; eauto.
+      assert (Y \notin L) as Fr by eauto.
+      specialize (H Y Fr).
+      eapply typing_regular in H. destruct H as [? [A ?]].
+      eapply A.
+    + false. eapply binds_empty_inv; eauto.
+    + eapply pt_all; eauto.
+    + apply_fresh pt_all as Y. eauto.
+      eapply sub_trans; eauto.
+      eapply sub_trans; eauto.
+      eapply sub_trans.
+      eapply sub_narrowing_empty. eauto. eauto. eapply H2. eauto.
+      assert (Y \notin L0) as Fr by eauto.
+      specialize (H10 Y Fr). simpl in H10. rewrite concat_empty_l in H10. eapply H10.
 Qed.
 
-Lemma typing_inv_tabs : forall E S10 S11 e1 T,
-  typing E (trm_tabs S10 S11 e1) T ->
-  forall U10 U11 U2, sub notrans E T (typ_all U10 U11 U2) -> sub oktrans E U10 U11 ->
-     sub oktrans E S10 U10 /\ sub oktrans E U11 S11
-  /\ exists S2, exists L, forall X, X \notin L ->
-     typing (E & X ~ bind_sub U10 U11) (e1 open_te_var X) (S2 open_tt_var X)
-     /\ sub oktrans (E & X ~ bind_sub U10 U11) (S2 open_tt_var X) (U2 open_tt_var X).
+Lemma possible_types_typing : forall v T,
+  typing empty v T -> value v ->
+  possible_types v T.
 Proof.
-  intros E S10 S11 e1 T H. gen_eq e: (trm_tabs S10 S11 e1). gen S10 S11 e1.
-  induction H; intros S10 S11 b EQ U10 U11 U2 Sub SubU; inversion EQ.
-  inversions Sub.
-  subst. splits.
-   apply* sub_reflexivity.
-   apply* sub_reflexivity.
-   exists U2 L.
-   intros Y Fr. splits.
-   apply H; assumption.
-   specialize (H Y Fr).
-   apply typing_regular in H.
-   apply* sub_reflexivity.
+  introv Ht Hv.
+  remember Ht as Hc. clear HeqHc.
+  remember empty as E. generalize HeqE. generalize Hc.
+  induction Ht; intros; subst; eauto; try solve [inversion Hv].
+  - eapply typing_regular in Hc. destruct Hc as [? [? Hc]].
+    inversion Hc; subst.
+    apply_fresh pt_arrow as y.
+    assert (y \notin L) as Fr by eauto.
+    specialize (H y Fr). rewrite concat_empty_l in H. eapply H.
+    eapply sub_reflexivity; eauto. eapply sub_reflexivity; eauto.
+  - eapply typing_regular in Hc. destruct Hc as [? [? Hc]].
+    inversion Hc; subst.
+    apply_fresh pt_all as Y.
+    assert (Y \notin L) as Fr by eauto.
+    specialize (H Y Fr). rewrite concat_empty_l in H. eapply H.
+    eapply sub_reflexivity; eauto. eapply sub_reflexivity; eauto.
+    eapply sub_reflexivity; eauto.
+    rewrite <- concat_empty_l. eauto.
+    assert (Y \notin L0) as Fr by eauto.
+    specialize (H9 Y Fr). rewrite concat_empty_l in H9. eapply H9.
+  - eapply possible_types_closure; eauto.
+    eapply sub_trans_pushback_empty; eauto.
+Qed.
+
+Lemma typing_inv_abs : forall S1 e1 T,
+  typing empty (trm_abs S1 e1) T ->
+  forall U1 U2, sub notrans empty T (typ_arrow U1 U2) ->
+     sub oktrans empty U1 S1
+  /\ exists S2, exists L, forall x, x \notin L ->
+     typing (x ~ bind_typ S1) (e1 open_ee_var x) S2 /\ sub oktrans empty S2 U2.
+Proof.
+  introv Typ.
+  remember (trm_abs S1 e1) as v.
+  assert (value v) as Hv. {
+    subst. eapply value_abs. eapply typing_regular in Typ. destruct Typ as [? [A ?]].
+    eapply A.
+  }
+  gen S1 e1.
+  assert (possible_types v T) as Hpt. {
+    eapply possible_types_typing; eauto.
+  }
+  clear Typ. clear Hv.
+  inversion Hpt; subst; introv Eqv Hsub; try solve [inversion Hsub].
+  inversion Hsub; subst. inversion Eqv; subst.
+  split.
+  eapply sub_trans; eauto.
+  eexists. exists L.
+  intros y Fr.
+  specialize (H y Fr).
+  split. eapply H.
+  eapply sub_trans; eauto.
+Qed.
+
+Lemma typing_inv_tabs : forall S10 S11 e1 T,
+  typing empty (trm_tabs S10 S11 e1) T ->
+  forall U10 U11 U2, sub notrans empty T (typ_all U10 U11 U2) -> sub oktrans empty U10 U11 ->
+     sub oktrans empty S10 U10 /\ sub oktrans empty U11 S11
+  /\ exists S2, exists L, forall X, X \notin L ->
+     typing (X ~ bind_sub U10 U11) (e1 open_te_var X) (S2 open_tt_var X)
+     /\ sub oktrans (X ~ bind_sub U10 U11) (S2 open_tt_var X) (U2 open_tt_var X).
+Proof.
+  introv Typ.
+  remember (trm_tabs S10 S11 e1) as v.
+  assert (value v) as Hv. {
+    subst. eapply value_tabs. eapply typing_regular in Typ. destruct Typ as [? [A ?]].
+    eapply A.
+  }
+  gen S10 S11 e1.
+  assert (possible_types v T) as Hpt. {
+    eapply possible_types_typing; eauto.
+  }
+  clear Typ. clear Hv.
+  inversion Hpt; subst; introv Eqv Hsub; try solve [inversion Hsub].
+  inversion Eqv; subst. inversion Hsub; subst; introv HsubU.
+  splits*. eexists. exists L. intros Y Fr. splits*.
+  specialize (H Y Fr). eapply typing_narrowing_empty; eauto.
+
   splits.
-   auto. auto.
-   exists T1. let L1 := gather_vars in exists L1.
-   intros Y Fr. splits.
-    apply_empty* (@typing_narrowing S10 S11). auto. auto.
-  auto* (@sub_transitivity T) sub_trans_ok sub_trans_pushback.
+  eapply sub_trans; eauto.
+  eapply sub_trans; eauto.
+  eexists. exists (L \u L0).
+  intros Y Fri.
+  assert (Y \notin L) as Fr by auto.
+  assert (Y \notin L0) as Fr0 by auto.
+  splits.
+  specialize (H Y Fr).
+  eapply typing_narrowing_empty.
+  eapply sub_trans. eapply H0. eauto.
+  eapply sub_trans. eauto. eauto.
+  eauto.
+  eauto.
+  specialize (H2 Y Fr). specialize (H12 Y Fr0). rewrite concat_empty_l in H12.
+  eapply sub_trans.
+  eapply sub_narrowing_empty. eauto. eauto. eapply H2. eapply H12.
 Qed.
 
 (* ********************************************************************** *)
@@ -1627,7 +1780,7 @@ Proof.
     pick_fresh X. forwards~ K: (P2 X). destruct K.
      rewrite* (@subst_ee_intro X).
      apply_empty (@typing_through_subst_ee V).
-       apply* (@typing_sub S2). apply_empty* sub_weakening.
+       apply* (@typing_sub S2). rewrite concat_empty_l. auto*. apply_empty* sub_weakening_empty.
        auto*.
   (* case: tapp *)
   inversions Red; try solve [ apply* typing_tapp ].
@@ -1638,7 +1791,7 @@ Proof.
      rewrite* (@subst_tt_intro X).
      erewrite <- map_empty.
      apply* (@typing_through_subst_te T0 T1).
-     rewrite concat_empty_r. rewrite concat_empty_l in *.
+     rewrite concat_empty_r.
      apply* typing_sub.
   (* case sub *)
   apply* typing_sub.
@@ -1656,7 +1809,7 @@ Proof.
   introv Val Typ. gen_eq E: (@empty bind).
   induction Typ; introv EQE;
     try solve [ inversion Val; congruence ].
-  apply sub_trans_pushback in H.
+  subst. apply sub_trans_pushback_empty in H.
   inversion H; subst; try solve [ congruence ].
   induction T; try solve [ congruence ].
   apply IHTyp; auto.
@@ -1671,7 +1824,7 @@ Proof.
   gen_eq T: (typ_arrow U1 U2). gen U1 U2.
   induction Typ; introv EQT EQE;
    try solve [ inversion Val | inversion EQT | eauto ].
-    subst. apply sub_trans_pushback in H. inversion H.
+    subst. apply sub_trans_pushback_empty in H. inversion H.
       apply value_not_bot in Typ; try assumption. congruence.
       false (binds_empty_inv H0).
       inversions H0. forwards*: IHTyp.
@@ -1685,7 +1838,7 @@ Proof.
   gen_eq T: (typ_all U0 U1 U2). gen U0 U1 U2.
   induction Typ; introv EQT EQE;
    try solve [ inversion Val | inversion EQT | eauto ].
-    subst. apply sub_trans_pushback in H. inversion H.
+    subst. apply sub_trans_pushback_empty in H. inversion H.
       apply value_not_bot in Typ; try assumption. congruence.
       false* binds_empty_inv.
       inversions H0. forwards*: IHTyp.
